merge props

type/merge.v
@@ -9,23 +9,163 @@ Require Import Coq.Init.Datatypes.
 Inductive Forall3 {A B C} : (A -> B -> C -> Prop) -> list A -> list B -> list C -> Prop := 
   | Forall3_nil : forall P, Forall3 P nil nil nil
   | Forall3_cons : forall P a xa b xb c xc, P a b c -> Forall3 P xa xb xc -> Forall3 P (a :: xa) (b :: xb) (c :: xc).
- 
 
 Inductive merge2 : ltt -> ltt -> ltt -> Prop := 
   | mrg_id : forall x, merge2 x x x
-  | mrg_bra : forall p xs ys IJ, Forall3 (fun u v w => 
-    (u = None /\ v = None /\ w = None) \/
-    (exists t, u = None /\ v = Some t /\ w = Some t) \/
-    (exists t, u = Some t /\ v = None /\ w = Some t) \/
-    (exists t, u = Some t /\ v = Some t /\ w = Some t)
-  ) xs ys IJ ->  merge2 (ltt_recv p xs) (ltt_recv p ys) (ltt_recv p IJ).
-
+  | mrg_bra : forall p xs ys IJ, 
+                Forall3 (fun u v w => 
+                  (u = None /\ v = None /\ w = None) \/
+                  (exists t, u = None /\ v = Some t /\ w = Some t) \/
+                  (exists t, u = Some t /\ v = None /\ w = Some t) \/
+                  (exists t, u = Some t /\ v = Some t /\ w = Some t)) xs ys IJ -> 
+              merge2 (ltt_recv p xs) (ltt_recv p ys) (ltt_recv p IJ).
 
 Inductive isMerge : ltt -> list (option ltt) -> Prop :=
   | matm : forall t, isMerge t (Some t :: nil)
   | mconsn : forall t xs, isMerge t xs -> isMerge t (None :: xs) 
   | mconss : forall t t' t'' xs, isMerge t xs -> merge2 t t' t'' -> isMerge t'' (Some t' :: xs). 
 
+Lemma merge2I_fst: forall l T p xs ys zs,
+  merge2 (ltt_recv p xs) (ltt_recv p ys) (ltt_recv p zs) ->
+  onth l zs = Some T ->
+  onth l xs = Some T \/  onth l xs = None.
+Proof. intro l.
+       induction l; intros.
+       - inversion H. subst. left. easy.
+       - subst. inversion H2. subst.
+         rewrite onthNil in H0. easy.
+         subst. simpl.
+         destruct H1 as [H1 | [H1 | H1]].
+         + right. easy.
+         + destruct H1 as (t, (H1a,(H1b,H1c))).
+           subst. simpl in H0. inversion H0. subst. right. easy.
+           destruct H1 as [H1 | H1].
+           ++ destruct H1 as (t, (H1a,(H1b,H1c))).
+              subst. left. easy.
+           ++ destruct H1 as (t, (H1a,(H1b,H1c))).
+              subst. simpl in H0. inversion H0. subst. left. easy.
+              case_eq xs; case_eq ys; case_eq zs; intros.
+              * subst. simpl in H0. easy.
+              * subst. simpl. right. easy.
+              * subst. simpl in H0. easy.
+              * subst. simpl in H0. simpl.
+                inversion H. subst. inversion H2.
+              * subst. simpl in H0. easy.
+              * subst. inversion H. subst. inversion H2.
+              * subst. simpl in H0. easy.
+              * subst. simpl. simpl in H0.
+                inversion H. subst. simpl in H0. left. easy. 
+                subst.
+                apply IHl with (p := p) (ys := l1) (zs := l0).
+                inversion H2. subst.
+                apply (mrg_bra p) in H10. easy. easy.
+Qed.
+
+Lemma merge2I_snd: forall l T p xs ys zs,
+  merge2 (ltt_recv p xs) (ltt_recv p ys) (ltt_recv p zs) ->
+  onth l zs = Some T ->
+  onth l ys = Some T \/  onth l ys = None.
+Proof. intro l.
+       induction l; intros.
+       - inversion H. subst. left. easy.
+       - subst. inversion H2. subst.
+         rewrite onthNil in H0. easy.
+         subst. simpl.
+         destruct H1 as [H1 | [H1 | H1]].
+         + right. easy.
+         + destruct H1 as (t, (H1a,(H1b,H1c))).
+           subst. simpl in H0. inversion H0. subst. left. easy.
+           destruct H1 as [H1 | H1].
+           ++ destruct H1 as (t, (H1a,(H1b,H1c))).
+              subst. right. easy.
+           ++ destruct H1 as (t, (H1a,(H1b,H1c))).
+              subst. simpl in H0. inversion H0. subst. left. easy.
+              case_eq xs; case_eq ys; case_eq zs; intros.
+              * subst. simpl in H0. easy.
+              * subst. simpl. right. easy.
+              * subst. simpl in H0. easy.
+              * subst. simpl in H0. simpl.
+                inversion H. subst. inversion H2.
+              * subst. simpl in H0. easy.
+              * subst. inversion H. subst. inversion H2.
+              * subst. simpl in H0. easy.
+              * subst. simpl. simpl in H0.
+                inversion H. subst. simpl in H0. left. easy. 
+                subst.
+                apply IHl with (p := p) (xs := l2) (zs := l0).
+                inversion H2. subst.
+                apply (mrg_bra p) in H10. easy. easy.
+Qed.
+
+Lemma merge2_fst: forall l T p xs ys zs,
+  merge2 (ltt_recv p xs) (ltt_recv p ys) (ltt_recv p zs) ->
+  onth l xs = Some T ->
+  onth l zs = Some T.
+Proof. intro l.
+       induction l; intros.
+       - inversion H. subst. easy.
+         subst. case_eq xs; case_eq ys; case_eq zs; intros.
+         * subst. simpl in H0. easy.
+         * subst. simpl in H0. easy.
+         * subst. inversion H.  subst. inversion H3. subst. easy.
+         * subst. simpl in H0. easy.
+         * subst. inversion H.  subst. inversion H3. subst. easy.
+         * subst. simpl in *. inversion H2. subst.
+           destruct H6 as [H6 | [H6 | H6]]. 
+           + easy.
+           + destruct H6 as (t, (H6a,(H6b,H6c))). inversion H6b. subst. easy.
+           + destruct H6 as [H6 | H6].
+             * destruct H6 as (t, (H6a,(H6b,H6c))). inversion H6b. subst. easy.
+             * destruct H6 as (t, (H6a,(H6b,H6c))). inversion H6b. subst. easy.
+       - subst. case_eq xs; case_eq ys; case_eq zs; intros.
+         * subst. simpl in H0. easy.
+         * subst. simpl in H0. easy.
+         * subst. simpl in *. inversion H. subst. inversion H2.
+         * subst. simpl in *. inversion H. subst. inversion H2.
+         * subst. simpl in *. inversion H. subst. inversion H2.
+         * subst. simpl in *. inversion H. subst. inversion H2.
+         * subst. simpl in *. inversion H. subst. inversion H2.
+         * subst. simpl in *.
+           inversion H. subst. easy. subst.
+           apply IHl with (p := p) (xs := l2) (ys := l1).
+           inversion H2. subst.
+           apply (mrg_bra p) in H10. easy. easy. 
+Qed.
+
+Lemma merge2_snd: forall l T p xs ys zs,
+  merge2 (ltt_recv p xs) (ltt_recv p ys) (ltt_recv p zs) ->
+  onth l ys = Some T ->
+  onth l zs = Some T.
+Proof. intro l.
+       induction l; intros.
+       - inversion H. subst. easy.
+         subst. case_eq xs; case_eq ys; case_eq zs; intros.
+         * subst. simpl in H0. easy.
+         * subst. simpl in H0. easy.
+         * subst. inversion H.  subst. inversion H3. subst. easy.
+         * subst. simpl in H0. easy.
+         * subst. inversion H.  subst. inversion H3. subst. easy.
+         * subst. simpl in *. inversion H2. subst.
+           destruct H6 as [H6 | [H6 | H6]]. 
+           + easy.
+           + destruct H6 as (t, (H6a,(H6b,H6c))). inversion H6b. subst. easy.
+           + destruct H6 as [H6 | H6].
+             * destruct H6 as (t, (H6a,(H6b,H6c))). easy.
+             * destruct H6 as (t, (H6a,(H6b,H6c))). inversion H6b. subst. easy.
+       - subst. case_eq xs; case_eq ys; case_eq zs; intros.
+         * subst. simpl in H0. easy.
+         * subst. simpl in H0. easy.
+         * subst. simpl in *. inversion H. subst. inversion H2.
+         * subst. simpl in *. inversion H. subst. inversion H2.
+         * subst. simpl in *. inversion H. subst. inversion H2.
+         * subst. simpl in *. inversion H. subst. inversion H2.
+         * subst. simpl in *. inversion H. subst. inversion H2.
+         * subst. simpl in *.
+           inversion H. subst. easy. subst.
+           apply IHl with (p := p) (xs := l2) (ys := l1).
+           inversion H2. subst.
+           apply (mrg_bra p) in H10. easy. easy. 
+Qed.
 
 Lemma _a_29_part_helper_recv : forall n ys1 x4 p ys,
     onth n ys1 = Some x4 ->
@@ -75,7 +215,6 @@ Proof. intro n.
          apply IHn. easy. easy.
 Qed.
 
-
 Lemma triv_merge : forall T T', isMerge T (Some T' :: nil) -> T = T'.
 Proof. intros.
        inversion H. subst. easy. subst.
@@ -121,36 +260,76 @@ Lemma merge_label_recv : forall Mp LQ' LQ0' T k l p,
           onth k Mp = Some (ltt_recv p LQ0') ->
           onth l LQ0' = Some T ->
           exists T', onth l LQ' = Some T'.
-Proof. intros Mp LQ' LQ0' T k.
-       revert Mp LQ' LQ0' T.
-       induction k; intros.
-       - inversion H. subst. simpl in H0.
-         inversion H0. subst. exists T. easy.
-         subst. simpl in H0. easy.
-         subst. simpl in H0. inversion H0. subst.
-         inversion H3. subst. exists T. easy.
-         subst. inversion H6. subst.
-         rewrite onthNil in H1. easy.
-         subst.
-         destruct H4. destruct H4 as (H4a, (H4b, H4c)).
-         subst.  
-
-Admitted.
+Proof. intros Mp.
+       induction Mp; intros.
+       - rewrite onthNil in H0. easy.
+       - subst.
+         inversion H. subst.
+         case_eq k; intros. subst. simpl in H0. inversion H0. subst.
+         exists T. easy.
+         subst. simpl in H0. rewrite onthNil in H0. easy.
+         subst. case_eq k; intros.
+         + subst. simpl in H0. easy.
+         + subst. simpl in H0.
+           specialize(IHMp LQ' LQ0' T n l p). apply IHMp; try easy.
+           subst. case_eq k; intros.
+           ++ subst. simpl in H0. inversion H0. subst.
+              inversion H6. subst. exists T. easy.
+              subst.
+              specialize(merge2_snd l T p xs LQ0' LQ' H6 H1); intro HF.
+              exists T. easy.
+           ++ subst. simpl in H0.
+              inversion H6. subst.
+              specialize(IHMp LQ' LQ0' T n l p). apply IHMp; try easy.
+              subst. inversion H. subst.
+              rewrite onthNil in H0. easy.
+              subst.
+              specialize(IHMp xs LQ0' T n l p H5 H0 H1).
+              destruct IHMp as (u,IHu).
+              exists u.
+              specialize(merge2_fst l u p xs ys LQ' H6 IHu); intro HF.
+              easy.
+Qed.
 
 Lemma merge_label_send : forall Mq LP' LP0' T k l q,
           isMerge (ltt_send q LP') Mq ->
           onth k Mq = Some (ltt_send q LP0') ->
           onth l LP0' = Some T ->
           exists T', onth l LP' = Some T'. 
-Admitted.
+Proof. intro Mq.
+       induction Mq; intros.
+       - rewrite onthNil in H0. easy.
+       - inversion H. subst. case_eq k; intros. subst. simpl in H0. inversion H0. subst.
+         exists T. easy.
+         subst. simpl in H0. rewrite onthNil in H0. easy.
+         subst. case_eq k; intros.
+         + subst. simpl in H0. easy. subst. simpl in H0.
+           specialize(IHMq LP' LP0' T n l q). apply IHMq; try easy.
+           subst. inversion H6. case_eq k; intros. subst. simpl in H0. inversion H0. subst.
+           inversion H6. subst. exists T. easy.
+           subst. simpl in H0.
+           apply IHMq with (LP0' := LP0') (T := T) (k := n) (q := q); easy.
+Qed.
 
 Lemma merge_label_sendb : forall ys0 LP LP' ST n l q,
       isMerge (ltt_send q LP) ys0 ->
       onth n ys0 = Some (ltt_send q LP') ->
       onth l LP = Some ST ->
       onth l LP' = Some ST.
-Admitted.
-
+Proof. intro ys0.
+       induction ys0; intros.
+       - rewrite onthNil in H0. easy.
+       - inversion H. subst. 
+         case_eq n; intros. subst. simpl in H0. inversion H0. subst. easy.
+         subst. simpl in H0. rewrite onthNil in H0. easy.
+         subst. case_eq n; intros. subst. simpl in H0. easy.
+         subst. simpl in H0.
+         apply IHys0 with (LP := LP) (n := n0) (q := q); easy.
+         subst. inversion H6. subst.
+         case_eq n; intros. subst. simpl in H0. inversion H0. subst. easy.
+         subst. simpl in H0.
+         apply IHys0 with (LP := LP) (n := n0) (q := q); easy.
+Qed.
 
 Lemma merge_constr : forall p LQ ys1 n,
           isMerge (ltt_recv p LQ) ys1 ->
